current progress

semantics/chorTypeScript.sml
@@ -8,9 +8,8 @@ val _ = new_theory "chorType";
 Inductive chorTypecheckOK:
 [~nil:] ∀ Γ Θ. chorTypecheckOK Γ Θ Nil
 [~com:] ∀ Γ Θ p1 v1 p2 v2 c. FLOOKUP Γ (v1,p1) = SOME strT ∧
-                             FLOOKUP Γ (v2,p2) = SOME strT ∧
                              ({p1;p2} ⊆ Θ) ∧ p1≠ p2 ∧
-                             chorTypecheckOK Γ Θ c ⇒
+                             chorTypecheckOK (Γ |+ ((v2,p2), strT)) Θ c ⇒
                              chorTypecheckOK Γ Θ (Com p1 v1 p2 v2 c)
 [~sel:] ∀ Γ Θ p1 p2 b c. ({p1;p2} ⊆ Θ) ∧ p1 ≠ p2 ∧ chorTypecheckOK Γ Θ c ⇒
                          chorTypecheckOK Γ Θ (Sel p1 b p2 c)
@@ -18,8 +17,7 @@ Inductive chorTypecheckOK:
                         chorTypecheckOK Γ Θ c1 ∧ chorTypecheckOK Γ Θ c2 ⇒
                         chorTypecheckOK Γ Θ (IfThen v p c1 c2)
 [~let:] ∀ Γ Θ v p e c ety. typecheck (localise Γ p) e ety ∧
-                           FLOOKUP Γ (v,p) = SOME ety ∧
-                           chorTypecheckOK Γ Θ c ⇒
+                           chorTypecheckOK (Γ |+ ((v,p), ety)) Θ c ⇒
                            chorTypecheckOK Γ Θ (Let v p e c)
 [~fix:] ∀ Γ Θ c dn. chorTypecheckOK Γ (Θ ∪ {dn}) c ⇒ chorTypecheckOK Γ Θ (Fix dn c)
 [~call:] ∀ Γ Θ dn. {dn} ⊆ Θ ⇒ chorTypecheckOK Γ Θ (Call dn)
