richerlang/envSemScript.sml
@@ -312,14 +312,25 @@ Proof
   gvs[]
 QED
 
+(*
 Theorem clock_eval_exp_result:
-  eval_exp cl1 E e = Value ev ∧ eval_exp cl2 E e = r ∧ r ≠ Timeout ⇒
+  ∀ cl1 cl2 E e ev r. eval_exp cl1 E e = Value ev ∧ eval_exp cl2 E e = r ∧ r ≠ Timeout ⇒
                       r = Value ev
 Proof
   rw[] >> Cases_on ‘cl1 ≤ cl2’
   >- (‘cl2 ≥ cl1’ by simp[] >> ‘eval_exp cl2 E e = Value ev’ by metis_tac[clock_value_increment]
       >> simp[])
   >> ‘cl1 ≥ cl2’ by simp[] >> Cases_on ‘eval_exp cl2 E e’ >> metis_tac[clock_increment]
+QED
+*)
+
+Theorem eval_exp_value_exn_false:
+  eval_exp c E e = Value ev ∧ eval_exp cl E e = Exn exn ⇒ F
+Proof
+  spose_not_then assume_tac >> Cases_on ‘c ≤ cl’
+  >- (‘cl ≥ c’ by simp[] >> ‘eval_exp cl E e = Value ev’ by metis_tac[clock_value_increment]>> gvs[])
+  >> ‘c ≥ cl’ by simp[] >> Cases_on ‘eval_exp cl E e’ >> gvs[clock_increment] >>
+  ‘c ≥ cl’ by simp[] >> ‘eval_exp c E e = Exn e'’ by metis_tac[clock_exn_increment]>> gvs[]
 QED
 
 Theorem clock_eval_exp_typeerr_false:
